# Conference 1 Micro Theory 250D2 

Jacob Hazen<br>material is not $100 \%$ my ideas jacobhazen1.github.io/

5 February 2024

## Random Variable

- Probability is about random variables (r.v.)
- A random variable is any "probabilistic" outcome.
- Flip of coin
- Height of someone randomly chosen in a population


## Sample Space \& Atoms

- r.v. take on values in a sample space discrete or continuous
- For example:
- The sample space of a toss of a coin is coin $\in\{H, T\}$
- Height of person: person $\in\{0, \infty\}$
- We call the values atoms


## Discrete Distributions

- A discrete distribution assigns a probability to every atom in the sample space:
- E.G. let $X \in\{H, T\}$ now

$$
\begin{aligned}
& P(X=H)=0.5 \\
& P(X=T)=0.5
\end{aligned}
$$

- Note: the entire state space must sum to 1

$$
\sum_{x} P(X=x)=1
$$

- Now is a good time to introduce an Event ( $X$ ) and a Outcome ( $x$ ).
- An Event is simply a subset of a sample space (S), in formal terms, $X \subseteq S$.
- Sum over part of the Discrete Space Dice:
- $P(D>3)=P(D=4)+P(D=5)+P(D=6)$


## Probability Theory: Bayes Rule

$$
P(A \text { and } B \mid B)=P(A \cap B \mid B)=P(A, B \mid B)=P(A \mid B)=\frac{P(A, B)}{P(B)}
$$

Note: The first two formula's starting from the left is just to for your notation. Specifically $P(A, B \mid B)=P(A \mid B)$ in the literature people remove the $B$ because it's standard/redundant, but it is important to understand the relationship.

$$
\begin{aligned}
P(A, B \mid B) & =\frac{P(A, B)}{P(B)} \\
P(A, B \mid B) P(B) & =P(A, B)
\end{aligned}
$$

Now Note:

$$
\begin{aligned}
P(A, B \mid A) & =\frac{P(A, B)}{P(A)} \\
P(A, B \mid A) P(A) & =P(A, B)
\end{aligned}
$$

Thus Bayes theorem is:

$$
P(A, B \mid A)=\frac{P(A, B \mid B) P(B)}{P(A)}
$$

Or in the standard notation where $P(A, B \mid B)=P(A \cap B \mid B)=P(A \mid B)$

$$
P(A \mid B)=\frac{P(B \mid A) P(A)}{P(B)}
$$

## Conditional Distributions

$$
P(X=x, Y=y \mid Y=y)=P(x \mid y)=\frac{P(x, y)}{P(y)}
$$

## Chain Rule

$$
P(X, Y)=P(X, Y) \frac{P(Y)}{P(Y)}=P(X, Y \mid Y) P(Y)
$$

Then in General:

$$
\begin{aligned}
P\left(X_{1}, \ldots, X_{N}\right) & =\prod_{n=1}^{N} P\left(X_{n} \mid X_{1}, \ldots, X_{n-1}\right) \\
& =\prod_{n=1}^{N} P\left(X_{n} \mid \cap_{j=1}^{n-1} X_{j}\right)
\end{aligned}
$$

## Marginalization

- Given a collection of R.V. we are only interested in a subset of them
- Lets compute $P(X)$ from joint distribution $P(X, Y, Z)$
- Marginalization allows us to compute this:

$$
P(X)=\sum_{y} \sum_{z} P(X, Y=y, Z=z)
$$

Sum over all the possible values that $Y$ and $Z$ can take in the joint distribution of $X, Y, Z$ gives us $P(X)$

Continuous

$$
f_{X}(x)=\int_{a}^{b} \int_{c}^{d} f(x, y, z) d x d z
$$

Where $x \in[a, b]$ and $y \in[c, d]$

Deriving above from Chain Rule:

$$
\begin{aligned}
\sum_{y} \sum_{z} P(x, y, z) & =P(y, z \mid x) P(x) \\
& =P(x) \sum_{y} \sum_{z} P(y, z \mid x) \\
& =P(x)
\end{aligned}
$$

Note: $\sum_{y} \sum_{z} P(y, z \mid x)=1$

Bayes Theorem using Marginalization and Chain Rule

$$
P(Y \mid X)=\frac{P(X \mid Y) P(Y)}{P(X)}
$$

$$
=\frac{P(X \mid Y) P(Y)}{\sum_{y} P(X \mid Y=y) P(Y=y)}
$$

Ok, this version of Bayes is a lot to take in but it is KEY to understanding how we can use the observable data to uncover the hidden distribution.

- $P(Y)$ is the prior distribution, in other words, the distribution we know already from the data.
- $P(Y \mid X)$ is the posterior distribution, in other words, we update future knowledge using our prior knowledge of the distribution (i.e $P(Y)$ ) given the new observed data $X$
Next is the $P(X)$, our data observed data comes in terms of data points, how do we estimate $P(X)$ from the data.
- Using the rules above $\sum_{y} P(X \mid Y=y) P(Y=y)=P(X)$, in other words, since we observe, $P(X \mid Y)$ using the chain rule + marginalization above we can get $P(X)$


## Example

Let $Y$ be a disease and $X$ be a symptom. From the distribution of the symptom given the disease $P(X \mid Y)$ and the probability of the disease $P(Y)$, we can compute the (more useful) distribution of the disease given the symptom $P(Y \mid X)$.

